

## 3.6 Derivatives of Logarithms

### 1 Derivative of $\ln(x)$

**Facts:**  $\frac{d}{dx}(\ln x) = \frac{1}{x}$       and       $\frac{d}{dx}[\ln(f(x))] = \frac{f'(x)}{f(x)}$       (Memorize this)

#### 1.0.1 Example:

Find the derivative of  $y = \ln(\sin x)$

---

#### 1.0.2 Example:

Find the derivative of  $y = x^3 \ln(x)$

---

#### 1.0.3 Example:

Find the derivative of  $y = \ln(x^3 \sin x)$

---

#### 1.0.4 Example:

Find the derivative of  $y = \cos x \ln(x^2)$

## 2 Derivative of other logarithms

**Facts:**  $\frac{d}{dx}(\log_b x) = \frac{1}{x \ln b}$       and       $\frac{d}{dx}[\log_b(f(x))] = \frac{f'(x)}{\ln b \cdot f(x)}$

### 2.0.1 Example:

Find the derivative of  $y = \log_2(x^2 + 5x + 1)$

---

## 3 Review of log rules

1.  $\log_a(M^N) = N \log_a(M)$
2.  $\log_a(MN) = \log_a M + \log_a N$
3.  $\log_a(M/N) = \log_a M - \log_a N$

We can use these rules to expand a complicated logarithm into several simpler logarithms.

### 3.0.1 Example:

$$\ln \left( \frac{xy^3}{z^4} \right) = \ln x + 3 \ln y - 4 \ln z$$

### 3.0.2 Examples:

Use the logarithm Rules to write as a sum or difference of two or more logarithms with no exponents:

$$\ln \left[ \frac{x^4(x-7)^5}{\sqrt{2x-9}} \right]$$

$$\log [x^6(x+7)^4]$$

### 3.0.3 Examples:

Use the logarithm Rules to write as a single logarithm:

$$2 \ln x^3 - 3 \ln(2x + 1) + \ln(x^2 + 1)$$

$$\ln(2x + 4) - 3 \ln(x + 3) - \frac{1}{2} \ln x$$

---

## 4 Using Log Rules to make derivatives easier

Suppose we are asked to find the derivative of  $y = \ln \left( \frac{x^2}{\sin x} \right)$ . It is HIGHLY preferable to use the log rules to expand it first, then take the derivative.

---

### 4.0.1 Example:

Find the derivative of  $y = \ln(x^3 \cos x \sqrt{3x^2 + 4})$

#### 4.0.2 Example:

Find the derivative of  $y = \ln \sqrt{\frac{5x-9}{1-x^2}}$

---

#### 4.0.3 Example:

Find the derivative of  $y = \ln \frac{x^2 e^{2x}}{x^2 + 1}$

---

## 5 Logarithmic Differentiation

### 5.1 Making hard derivatives easier

Taking the derivative of the function below would be painful. It would be easier if there were an  $\ln$  in front of the fraction.

$$y = \frac{x^2(1-x)^9}{x^4 \tan x}$$

So let's take the  $\ln$  of both sides.

$$\ln y = \ln \frac{x^2(1-x)^9}{x^4 \cos x}$$

Now we'll use implicit differentiation. Note that on the left, we have to use the chain rule. (The derivative of  $\ln y$  is  $\frac{y'}{y}$ .)

---

### 5.1.1 Example:

Use logarithmic differentiation to find the derivative of  $y = (1 + x + x^2)^4(x^2 - 4)^7$

### 5.1.2 Example:

Differentiate the function  $y = \frac{\sqrt{x}(x^3 + 9)}{(2x + 4)^3}$

---

## 5.2 Functions with $x$ both in the base and exponent

The simplest example of this is the function  $y = x^x$ . The only way we can find  $y'$  is by logarithmic differentiation.

### 5.2.1 Example:

Differentiate  $y = (\tan x)^x$

---

### 5.2.2 Example:

Find the derivative of  $y = (\ln x)^{\sin x}$